TransitionSystems/RegexProp.lean
@@ -1,0 +1,289 @@
+import Mathlib.Computability.RegularExpressions
+
+namespace TransitionSystems
+
+  @[reducible]
+  def RegexProp (α : Type) := RegularExpression (α → Bool)
+
+
+  namespace RegexProp
+
+    inductive PMatches {α} : RegexProp α → List α → Prop
+    | matchEpsilon : PMatches .epsilon []
+    | matchChar {p : α → Bool} {x : α} : p x → PMatches (.char p) [x]
+    | matchPlusLeft {r₁ r₂ : RegexProp α} {s : List α} :
+        PMatches r₁ s → PMatches (r₁ + r₂) s
+    | matchPlusRight {r₁ r₂} {s : List α} :
+        PMatches r₂ s → PMatches (r₁ + r₂) s
+    | matchComp {r₁ r₂ : RegexProp α} {s₁ s₂ : List α} :
+        PMatches r₁ s₁ → PMatches r₂ s₂ → PMatches (r₁ * r₂) (s₁ ++ s₂)
+    | matchStarNil (r : RegexProp α) : PMatches (.star r) []
+    | matchStarCons {r : RegexProp α} {x : α} {xs xs' : List α} :
+        PMatches r (x :: xs) → PMatches (.star r) xs' → PMatches (.star r) ((x :: xs) ++ xs')
+
+    @[reducible]
+    def charAny {α} : RegexProp α := .char (fun _ => true)
+
+    @[simp]
+    theorem pmatches_epsilon {α} : @PMatches α .epsilon [] := by constructor
+
+    @[simp]
+    theorem pmatches_char_cons {α} {p : α → Bool} {x : α} {xs : List α} :
+        PMatches (.char p) (x :: xs) ↔ p x ∧ xs = [] := by
+      apply Iff.intro <;> intro h
+      · cases h ; tauto
+      · cases xs <;> tauto
+
+    @[simp]
+    theorem pmatches_char_cons' {α} {p : α → Bool} {xs : List α} :
+        PMatches (.char p) xs ↔ ∃ x, p x ∧ xs = [x] := by
+      cases xs <;> simp
+      · intro h ; cases h
+      · rename_i x _ ; apply Iff.intro
+        · intro ; exists x ; tauto
+        · intro ⟨x', _⟩ ; cc
+
+
+    @[simp]
+    theorem pmatches_plus {α} {r₁ r₂ : RegexProp α} {xs : List α} :
+        PMatches (r₁ + r₂) xs ↔ PMatches r₁ xs ∨ PMatches r₂ xs := by
+      apply Iff.intro <;> intro h <;> cases h <;> tauto
+      apply PMatches.matchPlusRight ; assumption
+
+
+    theorem pmatches_comp {α} {r₁ r₂ : RegexProp α} {xs : List α} :
+        PMatches (r₁ * r₂) xs ↔ ∃ xs₁ xs₂,
+          xs = xs₁ ++ xs₂ ∧ PMatches r₁ xs₁ ∧ PMatches r₂ xs₂ := by
+      apply Iff.intro
+      · intro h ; cases h ; rename_i xs₁ xs₂ _ _ ; exists xs₁, xs₂
+      · intro ⟨xs₁, xs₂, happ, _, _⟩ ; rw [happ] ; constructor <;> assumption
+
+
+    @[simp]
+    theorem pmatches_comp_char_cons {α} {p : α → Bool} {r : RegexProp α} {x : α} {xs : List α} :
+        PMatches ((.char p) * r) (x :: xs) ↔ p x ∧ PMatches r xs := by
+      apply Iff.intro <;> simp [pmatches_comp]
+      · intros ; simp [*] at * ; cc
+      · intros ; exists [x], xs ; tauto
+
+    @[simp]
+    theorem pmatches_zero_comp {α} {r : RegexProp α} {xs : List α} : ¬ PMatches (0 * r) xs := by
+      intro ; contradiction
+
+    @[simp]
+    theorem pmatches_zero_plus {α} {r : RegexProp α} {xs : List α} : PMatches (0 + r) xs ↔ PMatches r xs := by
+      simp [pmatches_plus] ; intro ; contradiction
+
+    @[simp]
+    theorem pmatches_one_comp {α} {r : RegexProp α} {xs : List α} :
+        PMatches (1 * r) xs ↔ PMatches r xs := by
+      apply Iff.intro <;> intro h
+      · cases h ; rename_i h₁ h₂ ; cases h₁ ; exact h₂
+      · rw [←List.nil_append xs] ; tauto
+
+    /-
+      This approach to deciding RegexProps is almost 1:1 with
+      https://leanprover-community.github.io/mathlib4_docs/Mathlib/Computability/RegularExpressions.html#RegularExpression.deriv
+    -/
+
+    /-- `r.pderiv a` matches `x` if `r` matches `a :: x`, the Brzozowski derivative of `r` with respect
+  to `a`. -/
+    def pderiv {α} : RegexProp α → α → RegexProp α
+    | .zero, _ => .zero
+    | .epsilon, _ => .zero
+    | .char p, x => if p x then .epsilon else .zero
+    | .plus r₁ r₂, x => (pderiv r₁ x) + (pderiv r₂ x)
+    | .comp r₁ r₂, x =>
+        if r₁.matchEpsilon then (pderiv r₁ x * r₂ + pderiv r₂ x) else (pderiv r₁ x * r₂)
+    | .star r, x => pderiv r x * .star r
+
+
+    @[simp]
+    theorem pderiv_zero {α} (x : α) : pderiv 0 x = 0 := rfl
+
+    @[simp]
+    theorem pderiv_one {α} (x : α) : pderiv 1 x = 0 := rfl
+
+    @[simp]
+    theorem pderiv_char {α} (p : α → Bool) (x : α) :
+      pderiv (.char p) x = if p x then 1 else 0 := by simp [pderiv]
+
+    -- @[simp]
+    -- theorem pderiv_char_true {α} (p : α → Bool) (x : α) (h : p x = true) : pderiv (.char p) x = 1 :=
+    --   by simp [pderiv, h]
+
+    -- @[simp]
+    -- theorem pderiv_char_true' {α} (p : α → Prop) {_ : DecidablePred p} (x : α) (h : p x) :
+    --   pderiv (.char (fun x => decide (p x))) x = 1 := by simp [pderiv, h]
+
+    -- @[simp]
+    -- theorem pderiv_char_false {α} (p : α → Bool) (x : α) (h : p x = false) : pderiv (.char p) x = 0 :=
+    --   by simp [pderiv, h]
+
+    --     @[simp]
+    -- theorem pderiv_char_false' {α} (p : α → Prop) {_ : DecidablePred p} (x : α) (h : ¬ p x) :
+    --   pderiv (.char (fun x => decide (p x))) x = 0 := by simp [pderiv, h]
+
+    @[simp]
+    theorem pderiv_plus {α} (r₁ r₂ : RegexProp α) (x : α) :
+        pderiv (r₁ + r₂) x = pderiv r₁ x + pderiv r₂ x := rfl
+
+    @[simp]
+    theorem pderiv_star {α} (r : RegexProp α) (x : α) :
+        pderiv (.star r) x = (pderiv r x) * (.star r) := rfl
+
+
+    def rpmatch {α} : RegexProp α → List α → Bool
+    | r, [] => r.matchEpsilon
+    | r, x :: xs => rpmatch (r.pderiv x) xs
+
+    -- @[simp]
+    theorem rpmatch_nil {α} (r : RegexProp α) :
+        rpmatch r [] = r.matchEpsilon := rfl
+
+    @[simp]
+    theorem rpmatch_cons {α} (r : RegexProp α) (x : α) (xs : List α) :
+        rpmatch r (x :: xs) = rpmatch (r.pderiv x) xs := rfl
+
+    @[simp]
+    theorem rpmatch_zero {α} (xs : List α) : rpmatch 0 xs = false := by
+      induction xs <;> tauto
+
+    theorem one_rpmatch_iff {α} {xs : List α} :
+        rpmatch 1 xs ↔ xs = [] := by
+      cases xs <;> simp [rpmatch, RegularExpression.matchEpsilon]
+
+    theorem char_rpmatch_iff {α} {p : α → Bool} {xs : List α} :
+        rpmatch (.char p) xs ↔ ∃ x, xs = [x] ∧ p x := by
+      cases xs <;> simp [rpmatch, pderiv, RegularExpression.matchEpsilon]
+      rename_i x xs ; split <;> simp [*, one_rpmatch_iff] at *; tauto
+
+    theorem plus_rpmatch_iff {α} {r₁ r₂ : RegexProp α} {xs : List α} :
+        rpmatch (r₁ + r₂) xs ↔ rpmatch r₁ xs ∨ rpmatch r₂ xs := by
+      induction xs generalizing r₁ r₂ <;> simp [rpmatch, RegularExpression.matchEpsilon]
+      rename_i ih ; rw [ih]
+
+    theorem comp_rpmatch_iff {α} {r₁ r₂ : RegexProp α} {xs : List α} :
+        rpmatch (r₁ * r₂) xs ↔ ∃ xs₁ xs₂, xs = xs₁ ++ xs₂ ∧ rpmatch r₁ xs₁ ∧ rpmatch r₂ xs₂ := by
+      induction xs generalizing r₁ r₂ <;> simp [rpmatch, RegularExpression.matchEpsilon]
+      · apply Iff.intro ; tauto
+        intro ⟨xs₁, xs₂, ⟨h₁, h₂⟩, h⟩; rw [h₁, h₂] at h ; exact h
+      · rename_i x xs ih ; simp [pderiv] ; split
+        · apply Iff.intro
+          · rw [plus_rpmatch_iff, ih] ; intro h ; apply Or.elim h
+            · intro ⟨xs₁, xs₂, _⟩ ; exists x :: xs₁, xs₂ ; tauto
+            · intro ; exists [] ; tauto
+          · rw [plus_rpmatch_iff, ih] ; simp ; intros xs₁ xs₂ ; intros
+            cases xs₁ <;> simp [*] at *
+            · right ; rw [←rpmatch] ; cc
+            · left ; rename_i xs₁ _ _ ; exists xs₁, xs₂ ; cc
+        · rw [ih] ; apply Iff.intro <;> intro ⟨xs₁, xs₂, _⟩
+          · exists x :: xs₁, xs₂ ; tauto
+          · cases xs₁
+            · simp [rpmatch, *] at *
+            · rename_i xs₁ h ; simp at h ; exists xs₁, xs₂ ; cc
+
+    @[simp]
+    theorem rpmatch_star_nil {α} (r : RegexProp α) : rpmatch (.star r) [] = true := by rfl
+
+    theorem rpmatch_star_once {α} {r : RegexProp α} {xs : List α} :
+        rpmatch r xs → rpmatch (.star r) xs := by
+        cases xs <;> simp [rpmatch, comp_rpmatch_iff, RegularExpression.matchEpsilon]
+        case cons x xs => intro ; exists xs, [] ; simp ; tauto
+
+    theorem star_rpmatch_cons_rpmatch {α} {r : RegexProp α} {x : α} {xs : List α} :
+        rpmatch (.star r) (x :: xs) →
+        ∃ xs₁ xs₂, xs = xs₁ ++ xs₂ ∧ rpmatch r (x :: xs₁) ∧ rpmatch (.star r) xs₂ := by
+      simp [rpmatch, comp_rpmatch_iff]
+
+    theorem cons_rpmatch_star_rpmatch {α} {r : RegexProp α} {xs₁ xs₂ : List α} :
+        rpmatch r xs₁ → rpmatch (.star r) xs₂
+        → rpmatch (.star r) (xs₁ ++ xs₂) := by
+      cases xs₁ <;> simp [rpmatch, comp_rpmatch_iff]
+      rename_i x xs₁ ; intro h₁ h₂ ; exists xs₁, xs₂
+
+    theorem star_rpmatch_iff {α} {r : RegexProp α} {xs : List α} :
+        rpmatch (.star r) xs
+        ↔ ∃ xss : List (List α), xss.join = xs ∧ ∀ xs' ∈ xss, rpmatch r xs' := by
+      apply Iff.intro
+      · have ⟨n, hn⟩ : ∃ n, xs.length ≤ n := ⟨xs.length, le_rfl⟩
+        induction n generalizing xs <;> cases xs <;> simp at *
+        case zero.nil | succ.nil => exists [] ; tauto
+        case succ.cons n ih x xs =>
+          intro h
+          have ⟨xs₁, xs₂, hxs, h₁, h₂⟩ := star_rpmatch_cons_rpmatch h
+          have hn₂ : xs₂.length ≤ n := le_trans (by simp [*]) hn
+          have ⟨xss, hjoin, hxss⟩ := ih hn₂ h₂
+          exists (x :: xs₁) :: xss ; simp [*] ; exact hxss
+      · intro ⟨xss, hjoin, hxss⟩ ; induction xss generalizing xs
+        all_goals simp [*] at *
+        · rw [hjoin] ; exact rpmatch_star_nil r
+        · rw [←hjoin] ; rename_i ih ; exact cons_rpmatch_star_rpmatch hxss.1 (ih hxss.2)
+
+    theorem rpmatch_pmatches_iff {α} {r : RegexProp α} {xs : List α} :
+        rpmatch r xs = true ↔ PMatches r xs := by
+      induction r generalizing xs
+      case zero => simp ; intro h ; cases h
+      case epsilon =>
+        simp [one_rpmatch_iff] ; apply Iff.intro <;> intro h
+        · rw [h] ; constructor
+        · cases h ; rfl
+      case char x =>
+        simp [char_rpmatch_iff]
+        apply Iff.intro <;> intro ⟨x, _⟩ <;> exists x <;> tauto
+      case plus _ _ ihxs₁ ihxs₂ => simp [plus_rpmatch_iff, ihxs₁, ihxs₂]
+      case comp _ _ ihxs₁ ihxs₂ =>
+        simp [comp_rpmatch_iff, ihxs₁, ihxs₂] ; apply Iff.intro
+        · intro ⟨_, _, h, _, _⟩ ; rw [h] ; constructor <;> assumption
+        · intro h ; cases h ; tauto
+      case star r ih =>
+        simp [star_rpmatch_iff, ih] ; clear ih ; apply Iff.intro
+        · intro ⟨xss, hjoin, hxss⟩ ; induction xss generalizing xs
+          · simp at hjoin ; rw [hjoin] ; constructor
+          · simp at hjoin ; rw [←hjoin]
+            rename_i xs₁ xss ih ; cases xs₁ ; simp at *
+            · tauto
+            · constructor ; apply hxss ; tauto
+              exact ih (by rfl) (fun _ => by tauto)
+        · have ⟨n, hn⟩: exists n, xs.length ≤ n := ⟨xs.length, le_rfl⟩
+          intro h ; induction n generalizing xs <;> cases xs <;> simp at hn <;> cases h
+          case matchStarNil | matchStarNil =>
+            exists [] ; tauto
+          case matchStarCons n ih x xs₁ xs₂ _ _ =>
+            simp at hn ; specialize @ih xs₂ (by omega) (by assumption)
+            let ⟨xss, _, _⟩ := ih
+            exists (x :: xs₁) :: xss ; simpa [*]
+
+    instance instDecidablePMatches {α} (r : RegexProp α) : DecidablePred r.PMatches := fun _ =>
+      decidable_of_iff _ rpmatch_pmatches_iff
+
+
+    theorem pmatches_cons {α} {r : RegexProp α} {x : α} {xs : List α} :
+        PMatches r (x :: xs) ↔ PMatches (r.pderiv x) xs := by
+      apply Iff.trans (Iff.symm rpmatch_pmatches_iff)
+      apply Iff.trans _ (rpmatch_pmatches_iff)
+      rfl
+
+    @[simp]
+    theorem pmatches_star_nil {α} {r : RegexProp α} : PMatches (.star r) [] := by constructor
+
+    @[simp]
+    theorem pmatches_star_cons {α} {r : RegexProp α} {x : α} {xs : List α} :
+        PMatches (.star r) (x :: xs) ↔ PMatches (r.pderiv x * .star r) xs := pmatches_cons
+
+    theorem star_induction
+        {α} {r : RegexProp α} {p : List α → Prop} (xs : List α) (star_nil : p ∅)
+        (star_cons : ∀ xs₁ xs₂, PMatches r xs₁ → PMatches (.star r) xs₂ → p xs₂ → p (xs₁ ++ xs₂))
+        : PMatches (.star r) xs → p xs := by
+      have ⟨n, hn⟩ : exists n, xs.length ≤ n := ⟨_, le_rfl⟩
+      intro hxs; induction n generalizing xs
+      · simp at hn ; rw [hn] ; exact star_nil
+      · rename_i n ih ; cases xs <;> try simp [*]
+        cases' hxs ; rename_i x xs₁ xs₂ h₂ h₁
+        simp at hn
+        apply star_cons (x :: xs₁) xs₂ h₁ h₂
+        apply ih _ (by omega) h₂
+
+  end RegexProp
+
+end TransitionSystems
